Indexing Terms by their types in TyArith

Tapl/TyArith.lean
@@ -10,17 +10,17 @@ namespace Tapl.TyArith
     | nat: Ty
   deriving Repr, DecidableEq
 
-  inductive Term: Type where
-    | true: Term
-    | false: Term
-    | zero: Term
-    | pred: Term → Term
-    | succ: Term → Term
-    | isZero: Term → Term
-    | ite: Term → Term → Term → Term
+  inductive Term: Ty → Type where
+    | true: Term .bool
+    | false: Term .bool
+    | zero: Term .nat
+    | pred: Term .nat → Term .nat
+    | succ: Term .nat → Term .nat
+    | isZero: Term .nat → Term .bool
+    | ite: Term .bool → Term α → Term α → Term α
   deriving Repr, DecidableEq
 
-  def Term.typeOf: Term → Ty
+  def Term.typeOf: Term α → Ty
     | .true => .bool
     | .false => .bool
     | .zero => .nat
@@ -46,7 +46,7 @@ namespace Tapl.TyArith
           else sorry
         | _ => sorry
 
-  def Term.eval₁: Term → Term
+  def Term.eval₁: Term α → Term α
     | .true => .true
     | .false => .false
     | .zero => .zero
@@ -62,7 +62,7 @@ namespace Tapl.TyArith
     | .ite .false _ f => f
     | .ite c t f => .ite c.eval₁ t f
 
-  def Term.eval: Term → Term
+  def Term.eval: Term α → Term α
     | .true => .true
     | .false => .false
     | .zero => .zero
@@ -82,71 +82,61 @@ namespace Tapl.TyArith
         | .false => f.eval
         | _ => sorry
 
-  inductive TypeOf: Term → Ty → Prop where
-    | true: TypeOf Term.true Ty.bool
-    | false: TypeOf Term.false Ty.bool
-    | zero: TypeOf Term.zero Ty.nat
-    | pred (n: Term): TypeOf n Ty.nat → TypeOf n.pred Ty.nat
-    | succ (n: Term): TypeOf n Ty.nat → TypeOf n.succ Ty.nat
-    | isZero (n: Term): TypeOf n Ty.nat → TypeOf n.isZero Ty.nat
-    | ite (c t f: Term) (α: Ty): TypeOf c Ty.bool → TypeOf t α → TypeOf f α → TypeOf (.ite c t f) α
+  inductive TypeOf: Term α → Ty → Prop where
+    | true: TypeOf Term.true .bool
+    | false: TypeOf Term.false .bool
+    | zero: TypeOf Term.zero .nat
+    | pred (n: Term .nat): TypeOf n.pred .nat
+    | succ (n: Term .nat): TypeOf n.succ .nat
+    | isZero (n: Term .nat): TypeOf n .nat → TypeOf n.isZero .nat
+    | ite (c: Term .bool) (t f: Term α): TypeOf (.ite c t f) α
 
-  inductive Numeric: Term → Prop where
+  inductive Numeric: Term .nat → Prop where
     | zero: Numeric Term.zero
-    | succ: ∀ nv: Term, Numeric nv → Numeric nv.succ
+    | succ: ∀ nv: Term .nat, Numeric nv → Numeric nv.succ
 
-  inductive Value: Term → Prop where
-    | numeric: ∀ nv: Term, Numeric nv → Value nv
+  inductive Value: Term α → Prop where
+    | numeric: ∀ nv: Term .nat, Numeric nv → Value nv
     | true: Value Term.true
     | false: Value Term.false
 
-  inductive Eval₁: Term → Term → Prop where
-    | iteTrue: ∀ t f: Term, Eval₁ (.ite .true t f) t
-    | iteFalse: ∀ t f: Term, Eval₁ (.ite .false t f) f
-    | ite: ∀ c₁ c₂ t f: Term, Eval₁ c₁ c₂ → Eval₁ (.ite c₁ t f) (.ite c₂ t f)
-    | succ: ∀ t₁ t₂: Term, Eval₁ t₁ t₂ → Eval₁ t₁.succ t₂.succ
+  inductive Eval₁: Term α → Term α → Prop where
+    | iteTrue: ∀ t f: Term α , Eval₁ (.ite .true t f) t
+    | iteFalse: ∀ t f: Term α, Eval₁ (.ite .false t f) f
+    | ite: ∀ c₁ c₂: Term .bool, ∀ t f: Term α, Eval₁ c₁ c₂ → Eval₁ (.ite c₁ t f) (.ite c₂ t f)
+    | succ: ∀ t₁ t₂: Term .nat, Eval₁ t₁ t₂ → Eval₁ t₁.succ t₂.succ
     | predZero: Eval₁ Term.zero.pred .zero
-    | predSucc: ∀ t: Term, Numeric t → Eval₁ t.succ.pred t
-    | pred: ∀ t₁ t₂: Term, Eval₁ t₁ t₂ → Eval₁ t₁.pred t₂.pred
+    | predSucc: ∀ t: Term .nat, Numeric t → Eval₁ t.succ.pred t
+    | pred: ∀ t₁ t₂: Term .nat, Eval₁ t₁ t₂ → Eval₁ t₁.pred t₂.pred
     | isZeroZero: Eval₁ Term.zero.isZero .true
-    | isZeroSucc: ∀ t: Term, Numeric t → Eval₁ t.succ.isZero .false
-    | isZero: ∀ t₁ t₂: Term, Eval₁ t₁ t₂ → Eval₁ t₁isZero t₂.isZero
+    | isZeroSucc: ∀ t: Term .nat, Numeric t → Eval₁ t.succ.isZero .false
+    | isZero: ∀ t₁ t₂: Term .nat, Eval₁ t₁ t₂ → Eval₁ t₁isZero t₂.isZero
 
-  inductive Eval: Term → Term → Prop where
-    | iteTrue: ∀ c t₁ t₂ f: Term, Eval c Term.true → Value t₁ → Eval t₁ t₂ → Eval (.ite c t₁ f) t₂
-    | iteFalse: ∀ c t f₁ f₂: Term, Eval c Term.false → Value f₂ → Eval f₁ f₂ → Eval (.ite c t f₁) f₂
-    | succ: ∀ t₁ t₂: Term, Numeric t₂ → Eval t₁ t₂ → Eval t₁.succ t₂.succ
-    | predZero: ∀ t: Term, Eval t Term.zero → Eval t.pred Term.zero
-    | predSucc: ∀ t₁ t₂: Term, Numeric t₂ → Eval t₁ t₂.succ → Eval t₁.pred t₂
-    | isZeroZero: ∀ t₁: Term, Eval t₁ .zero → Eval t₁.isZero .true
-    | isZeroSucc: ∀ t₁ t₂: Term, Numeric t₂ → Eval t₁ t₂.succ → Eval t₁.isZero .false
+  inductive Eval: Term α → Term α → Prop where
+    | iteTrue: ∀ c: Term .bool, ∀ t₁ t₂ f: Term α, Eval c Term.true → Value t₁ → Eval t₁ t₂ → Eval (.ite c t₁ f) t₂
+    | iteFalse: ∀ c: Term .bool, ∀ t f₁ f₂: Term α, Eval c Term.false → Value f₂ → Eval f₁ f₂ → Eval (.ite c t f₁) f₂
+    | succ: ∀ t₁ t₂: Term .nat, Numeric t₂ → Eval t₁ t₂ → Eval t₁.succ t₂.succ
+    | predZero: ∀ t: Term .nat, Eval t Term.zero → Eval t.pred Term.zero
+    | predSucc: ∀ t₁ t₂: Term .nat, Numeric t₂ → Eval t₁ t₂.succ → Eval t₁.pred t₂
+    | isZeroZero: ∀ t₁: Term .nat, Eval t₁ .zero → Eval t₁.isZero .true
+    | isZeroSucc: ∀ t₁ t₂: Term .nat, Numeric t₂ → Eval t₁ t₂.succ → Eval t₁.isZero .false
 
-  theorem typeOf_typeOf: ∀ t: Term, ∀ ty: Ty, TypeOf t ty ↔ t.typeOf = ty := sorry
+  theorem typeOf_typeOf: ∀ t: Term α, TypeOf t α ↔ t.typeOf = α := sorry
 
-  theorem eval₁_eval₁: ∀ t₁ t₂: Term, Eval₁ t₁ t₂ ↔ t₁.eval₁ = t₂ := sorry
+  theorem eval₁_eval₁: ∀ t₁ t₂: Term α, Eval₁ t₁ t₂ ↔ t₁.eval₁ = t₂ := sorry
 
-  theorem eval_eval: ∀ t₁ t₂: Term, Eval t₁ t₂ ↔ t₁.eval = t₂.eval := sorry
+  theorem eval_eval: ∀ t₁ t₂: Term α, Eval t₁ t₂ ↔ t₁.eval = t₂.eval := sorry
 
-  theorem eval_rtc_eval₁: ∀ t₁ t₂: Term, RTC Eval₁ t₁ t₂ ↔ Eval t₁ t₂ := sorry
+  theorem eval_rtc_eval₁: ∀ t₁ t₂: Term α , RTC Eval₁ t₁ t₂ ↔ Eval t₁ t₂ := sorry
 
-  theorem ty_uniq /-(t: Term) (ty₁ ty₂: Ty)-/ (h₁: TypeOf t ty₁) (h₂: TypeOf t ty₂): ty₁ = ty₂ := by
-    cases h₁ with
-      | true => cases h₂ <;> rfl
-      | false => cases h₂ <;> rfl
-      | zero => cases h₂ <;> rfl
-      | pred n h => cases h₂ <;> rfl
-      | succ n h => cases h₂ <;> rfl
-      | isZero n h => cases h₂ <;> rfl
-      | ite c t f ty h₁ h₂ h₃ =>
-        cases h₂ with
-          | ite c₁ t₂ f₁ ty₁ h₄ h₅ h₆ => sorry
-          | _ => sorry
+  theorem ty_uniq (h₁: TypeOf t α) (h₂: TypeOf t β): α = β := by
+    cases h₁ <;> cases h₂ <;> rfl
 
   theorem ty_deriv_uniq: True := sorry
 
-  theorem canonical_forms₁: ∀ t: Term, Value t → TypeOf t Ty.bool → v = Term.true ∨ v = Term.false := sorry
-  theorem canonical_forms₂: ∀ t: Term, Value t → TypeOf t Ty.nat → Numeric v := sorry
+  theorem canonical_forms₁: ∀ t: Term .bool, Value t → v = Term.true ∨ v = Term.false := sorry
+  theorem canonical_forms₂: ∀ t: Term .nat, Value t → Numeric v := sorry
 
-  theorem TypeOf.progress: ∀ t₁: Term, ∀ ty: Ty, TypeOf t₁ ty → Value t₁ ∨ ∃ t₂: Term, Eval₁ t₁ t₂ := sorry
-  theorem TypeOf.preservation: ∀ t₁ t₂: Term, ∀ ty: Ty, TypeOf t₁ ty → Eval₁ t₁ t₂ → TypeOf t₂ ty := sorry
+  theorem TypeOf.progress: ∀ t₁: Term α, TypeOf t₁ α → Value t₁ ∨ ∃ t₂: Term α, Eval₁ t₁ t₂ := sorry
+  theorem TypeOf.preservation: ∀ t₁ t₂: Term α, Eval₁ t₁ t₂ → TypeOf t₂ α := sorry
 end Tapl.TyArith
